Started rewriting SpecM.v based on fixtrees, and got as far as defining CallS

theories/Ref/SpecM.v
@@ -14,6 +14,7 @@ From EnTree Require Import
      Ref.Padded
      Ref.EnTreeSpecDefinition
      Ref.MRecSpec
+     Ref.FixTree
 .
 From Coq Require Import
   Arith.Arith
@@ -34,1200 +35,10 @@ Import Monads.
 Import ProperNotations.
 
 
-(* Examples of higher-order functions we want to write *)
-Section HOExamples.
-
-Context M `{Monad M}.
-
-(* An inconsistent fix, used to write our examples with the least fuss *)
-Variable fixM : forall {A B}, ((A -> M B) -> A -> M B) -> A -> M B.
-Variable fixM2 : forall {A B C}, ((A -> B -> M C) -> A -> B -> M C) -> A -> B -> M C.
-
-Definition incrStream (str : nat -> M nat) n : M nat :=
-  bind (str n) (fun x => ret (x + 1)).
-
-Definition foo : (nat -> M nat) -> nat -> M nat :=
-  fixM2 (fun rec str n =>
-          match n with
-          | 0 => str 0
-          | S n' => rec (rec (incrStream str)) n'
-          end).
-
-Definition fibMap : (nat -> M nat) -> nat -> M nat :=
-  fixM2 (fun rec str n =>
-           match n with
-           | 0 => str 0
-           | S 0 => bind (rec str 0) (fun x => ret (x + 1))
-           | S (S n') =>
-               bind (rec str n')
-                 (fun x =>
-                    bind (rec str (S n'))
-                         (fun y => ret (x + y)))
-           end).
-
-End HOExamples.
-
-
-(** Event types **)
-
-(* An event type = a type of events plus their return types *)
-Polymorphic Record EvType@{u} : Type :=
-  { evTypeType :> Type@{u};
-    evRetType : EncodingType evTypeType }.
-
-Global Instance EncodingType_EvType (ET:EvType) : EncodingType ET :=
-  evRetType ET.
-
-
-(** Utilities for nat-indexed types, i.e., types indexed by "levels" **)
-
-(* Apply a level-incrementing function to increment from level 0 *)
-Fixpoint levelIncFrom0 (A : nat -> Type@{entree_u}) (incA : forall n, A n -> A (S n))
-  n (a : A 0) : A n :=
-  match n with
-  | 0 => a
-  | S n' => incA n' (levelIncFrom0 A incA n' a)
-  end.
-
-(* Apply a level-incrementing function multiple times, adding on the left *)
-Fixpoint levelAddL (A : nat -> Type@{entree_u}) (incA : forall n, A n -> A (S n))
-  n m (a : A m) : A (n + m) :=
-  match n return A (n + m) with
-  | 0 => a
-  | S n' => incA (n' + m) (levelAddL A incA n' m a)
-  end.
-
-(* Apply a level-incrementing function multiple times, adding on the right *)
-Fixpoint levelAddR n :
-  forall (A : nat -> Type@{entree_u}) (incA : forall n, A n -> A (S n)) m,
-    A n -> A (n + m) :=
-  match n return forall A incA m, A n -> A (n + m) with
-  | 0 => fun A incA m a => levelIncFrom0 A incA m a
-  | S n' =>
-      fun A incA m a =>
-        levelAddR n' (fun lvl => A (S lvl)) (fun lvl => incA (S lvl)) m a
-  end.
-
-(* Lift the level m of a type to the level max n m with a new level n on the left *)
-Fixpoint levelMaxL n m :
-  forall (A : nat -> Type@{entree_u}) (incA : forall n, A n -> A (S n)),
-    A m -> A (max n m) :=
-  match n return forall A incA, A m -> A (max n m) with
-  | 0 => fun _ _ a => a
-  | S n' =>
-      match m return forall A incA, A m -> A (max (S n') m) with
-      | 0 => fun A incA a => levelIncFrom0 A incA (S n') a
-      | S m' =>
-          fun A incA a =>
-            levelMaxL n' m' (fun lvl => A (S lvl)) (fun lvl => incA (S lvl)) a
-      end
-  end.
-
-(* Lift the level n of a type to the level max n m with a new level m on the right *)
-Fixpoint levelMaxR n m :
-  forall (A : nat -> Type@{entree_u}) (incA : forall n, A n -> A (S n)),
-    A n -> A (max n m) :=
-  match n return forall A incA, A n -> A (max n m) with
-  | 0 => fun A incA a => levelIncFrom0 A incA m a
-  | S n' =>
-      match m return forall A incA, A (S n') -> A (max (S n') m) with
-      | 0 => fun _ _ a => a
-      | S m' =>
-          fun A incA a =>
-            levelMaxR n' m' (fun lvl => A (S lvl)) (fun lvl => incA (S lvl)) a
-      end
-  end.
-
-Lemma elimLevelIncFrom0 A incA n B (f : forall n, A n -> B) :
-  (forall n a, f n a = f (S n) (incA n a)) ->
-  forall a, f n (levelIncFrom0 A incA n a) = f 0 a.
-Proof.
-  intros; induction n.
-  - reflexivity.
-  - simpl. rewrite <- H. apply IHn.
-Qed.
-
-Lemma elimLevelMaxL n m A incA B (f : forall n, A n -> B) :
-  (forall n a, f n a = f (S n) (incA n a)) ->
-  forall a, f (max n m) (levelMaxL n m A incA a) = f m a.
-Proof.
-  revert m A incA B f; induction n; intros; [ | destruct m ].
-  - reflexivity.
-  - apply elimLevelIncFrom0. assumption.
-  - apply (IHn m (fun lvl : nat => A (S lvl)) (fun lvl : nat => incA (S lvl))
-             B (fun n => f (S n))).
-    intros. apply H.
-Qed.
-
-Lemma elimLevelMaxR n m A incA B (f : forall n, A n -> B) :
-  (forall n a, f n a = f (S n) (incA n a)) ->
-  forall a, f (max n m) (levelMaxR n m A incA a) = f n a.
-Proof.
-  revert m A incA B f; induction n; intros; [ | destruct m ].
-  - apply elimLevelIncFrom0. assumption.
-  - reflexivity.
-  - apply (IHn m (fun lvl : nat => A (S lvl)) (fun lvl : nat => incA (S lvl))
-             B (fun n => f (S n))).
-    intros. apply H.
-Qed.
-
-(* Lift the level of a type to a level that is at least as big *)
-Program Definition levelLift A incA n m (l: n <= m) (a:A n) : A m :=
-  eq_rect _ A (levelAddL A incA (m - n) n a) _ _.
-Next Obligation.
-  rewrite Nat.add_comm. apply le_plus_minus_r. assumption.
-Defined.
-
-(* Map a level-polymorphic function over an object at a given level *)
-Definition levelMap A B (f : forall n:nat, A n -> B n) (a: { n & A n })
-  : { n & B n } :=
-  existT B (projT1 a) (f (projT1 a) (projT2 a)).
-
-(* Apply a level-polymorphic function to combine to level objects, incrementing
-their levels if necessary *)
-Definition levelCombine (A B C : nat -> Type@{entree_u}) incA incB
-  (f : forall n, A n -> B n -> C n) (a : { n & A n}) (b : { n & B n})
-  : { n & C n } :=
-  existT C
-    (max (projT1 a) (projT1 b))
-    (f (max (projT1 a) (projT1 b))
-       (levelMaxR (projT1 a) (projT1 b) A incA (projT2 a))
-       (levelMaxL (projT1 a) (projT1 b) B incB (projT2 b))).
-
-(* Move a successor from the type functor to the level argument *)
-Definition levelIncr (A : nat -> Type@{entree_u}) (a : { n & A (S n) })
-  : { n & A n } :=
-  existT A (S (projT1 a)) (projT2 a).
-
-(* Ensure the level of an object is at least some given lvl by mapping the
-object to the supremum of lvl and its current level *)
-Definition levelSup A incA lvl (a : { n & A n }) : { n & A n } :=
-  existT A (max (projT1 a) lvl)
-    (levelMaxR (projT1 a) lvl A incA (projT2 a)).
-
-(* An object whose level has been explicitly lifted to n *)
-Inductive Lifted (A : nat -> Type@{entree_u}) lvl : Type@{entree_u} :=
-| MkLifted lvl' (le : lvl' <= lvl) (a : A lvl').
-
-Definition mkLifted (A : nat -> Type@{entree_u}) lvl (a:A lvl) : Lifted A lvl :=
-  MkLifted A lvl lvl (le_n lvl) a.
-
-(* Inject from { n & A n } into a lifted type *)
-Definition injLifted (A : nat -> Type@{entree_u}) (a : { n & A n })
-  : Lifted A (projT1 a) :=
-  mkLifted A (projT1 a) (projT2 a).
-
-(* Increment the level of a Lifted object *)
-Definition incLifted A lvl (l: Lifted A lvl) : Lifted A (S lvl) :=
-  match l with
-  | MkLifted _ _ lvl' le a => MkLifted A (S lvl) lvl' (le_S lvl' lvl le) a
-  end.
-
-(* Lift the level of a Lifted object *)
-Definition liftLifted A lvl lvl' (leq : lvl <= lvl') (l: Lifted A lvl)
-  : Lifted A lvl' :=
-  match l with
-  | MkLifted _ _ lvl'' leq' a =>
-      MkLifted A lvl' lvl'' (le_trans _ _ _ leq' leq) a
-  end.
-
-(* Map a Lifted object back to an object with a level *)
-Definition elimLifted A lvl (l: Lifted A lvl) : { n & A n } :=
-  match l with
-  | MkLifted _ _ lvl' le a => existT A lvl' a
-  end.
-
-(* Incrementing the level of a Lifted does not change what it eliminates to *)
-Definition elimIncLiftedEq A lvl l :
-  elimLifted A (S lvl) (incLifted A lvl l) = elimLifted A lvl l :=
-  match l return elimLifted A (S lvl) (incLifted A lvl l) = elimLifted A lvl l with
-  | MkLifted _ _ lvl' le a => eq_refl (existT A lvl' a)
-  end.
-
-(* Make a Lifted with an existentially quantified level from an { n & A n } *)
-Definition mkExLifted (A : nat -> Type@{entree_u}) (a : { n & A n })
-  : { n & Lifted A n } :=
-  existT (Lifted A) (projT1 a) (mkLifted A (projT1 a) (projT2 a)).
-
-(* Combine two Lifted with existentially quantified levels *)
-Definition exLiftedCombine A B C
-  (f : forall n, Lifted A n -> Lifted B n -> C n)
-  (a : { n & Lifted A n}) (b : { n & Lifted B n})
-  : { n & C n } :=
-  existT C
-    (max (projT1 a) (projT1 b))
-    (f (max (projT1 a) (projT1 b))
-       (liftLifted A (projT1 a) (max (projT1 a) (projT1 b))
-          (Nat.le_max_l (projT1 a) (projT1 b))
-          (projT2 a))
-       (liftLifted B (projT1 b) (max (projT1 a) (projT1 b))
-          (Nat.le_max_r (projT1 a) (projT1 b))
-          (projT2 b))).
-
-
-(** Binary functors that preserve colimits **)
-
-(* The class of binary functors that preserve countable colimits, i.e., such
-that F A B is a colimit of countably many types whenever A and B are both
-colimits of countably many types. Since the type { n & A n } is always a colimit
-and colimits are unique up to isomorphism, this is equivalent to saying that F
-of two types of this form is isomorphic to a type of this form. We call the
-morphism to this colimit type "fmapMax2" because the first projection
-intuitively gives the maximum level contained in the object. *)
-Class ColimFunctor2 (F : Type@{entree_u} -> Type@{entree_u} -> Type@{entree_u}) :=
-  { fmap2 : forall A1 A2 B1 B2, (A1 -> A2) -> (B1 -> B2) -> F A1 B1 -> F A2 B2;
-    fmapMax2 : forall (A B : nat -> Type@{entree_u}),
-      (forall n, A n -> A (S n)) -> (forall n, B n -> B (S n)) ->
-      F { n:nat & A n} { n:nat & B n} ->
-      { n & F (A n) (B n) };
-    fmap2Proper : forall A1 A2 B1 B2,
-      Proper ((eq ==> eq) ==> (eq ==> eq) ==> eq ==> eq) (fmap2 A1 A2 B1 B2);
-    fmap2Id : forall A B fab, fmap2 A A B B (fun x => x) (fun x => x) fab = fab;
-    fmap2Comp : forall A1 A2 A3 B1 B2 B3 f1 f2 g1 g2 fab,
-      fmap2 A2 A3 B2 B3 f2 g2 (fmap2 A1 A2 B1 B2 f1 g1 fab) =
-        fmap2 A1 A3 B1 B3 (fun x => f2 (f1 x)) (fun x => g2 (g1 x)) fab;
-    fmapMax2Eq :
-    forall A B C D incA incB (f: forall n, A n -> C) (g: forall n, B n -> D) fab,
-      (forall n a, f n a = f (S n) (incA n a)) ->
-      (forall n b, g n b = g (S n) (incB n b)) ->
-      fmap2
-        (A (projT1 (fmapMax2 A B incA incB fab))) C
-        (B (projT1 (fmapMax2 A B incA incB fab))) D
-        (f (projT1 (fmapMax2 A B incA incB fab)))
-        (g (projT1 (fmapMax2 A B incA incB fab)))
-        (projT2 (fmapMax2 A B incA incB fab))
-      =
-        fmap2 { n & A n } C { n & B n } D
-          (fun a => f (projT1 a) (projT2 a))
-          (fun b => g (projT1 b) (projT2 b))
-          fab;
-  }.
-
-
-(* The constant functor preserves colimits *)
-#[global] Program Instance Const_ColimFunctor2 T : ColimFunctor2 (fun _ _ => T) :=
-  {|
-    fmap2 := fun _ _ _ _ f g (t:T) => t;
-    fmapMax2 := fun A B _ _ (t:T) => existT _ 0 t
-  |}.
-Next Obligation.
-  repeat intro. assumption.
-Defined.
-
-
-(* The pair functor preserves colimits *)
-#[global]
-Program Instance Pair_ColimFunctor2 : ColimFunctor2 (fun A B => prod A B) :=
-  {|
-    fmap2 := fun _ _ _ _ f g p => (f (fst p), g (snd p));
-    fmapMax2 :=
-      fun A B incA incB p =>
-        levelCombine _ _ _ incA incB (fun _ a b => (a, b)) (fst p) (snd p);
-  |}.
-Next Obligation.
-  repeat intro. f_equal.
-  - apply H; f_equal; assumption.
-  - apply H0; f_equal; assumption.
-Defined.
-Next Obligation.
-  simpl. f_equal; [ apply elimLevelMaxR | apply elimLevelMaxL ]; assumption.
-Defined.
-
-
-(* The sum functor preserves colimits (FIXME: implement this!) *)
-#[global]
-Program Instance Sum_ColimFunctor2 : ColimFunctor2 (fun A B => sum A B) :=
-  {|
-    fmap2 := fun _ _ _ _ f g s =>
-               match s with | inl a => inl (f a) | inr b => inr (g b) end;
-  |}.
-Next Obligation.
-Admitted.
-Next Obligation.
-Admitted.
-Next Obligation.
-Admitted.
-Next Obligation.
-Admitted.
-Next Obligation.
-Admitted.
-
-
-(* The Vector functor preserves colimits (FIXME: implement this!) *)
-#[global]
-Program Instance Vec_ColimFunctor2 n : ColimFunctor2 (fun A _ => VectorDef.t A n) :=
-  {| 
-    fmap2 := fun _ _ _ _ f _ v => VectorDef.map f v;
-  |}.
-Next Obligation.
-Admitted.
-Next Obligation.
-Admitted.
-Next Obligation.
-Admitted.
-Next Obligation.
-Admitted.
-Next Obligation.
-Admitted.
-
-
-#[global]
-Program Instance Compose_ColimFunctor2 F G H
-  `{ColimFunctor2 F} `{ColimFunctor2 G} `{ColimFunctor2 H}
-  : ColimFunctor2 (fun A B => F (G A B) (H A B)) :=
-  {|
-    fmap2 := fun A B C D f g (x:F (G A C) (H A C)) =>
-                    fmap2 (G A C) (G B D) (H A C) (H B D)
-                               (fmap2 A B C D f g)
-                               (fmap2 A B C D f g) x;
-    fmapMax2 :=
-      fun A B incA incB x =>
-        fmapMax2
-          (F:=F)
-          (fun n => G (A n) (B n))
-          (fun n => H (A n) (B n))
-          (fun n => fmap2 (A n) (A (S n)) (B n) (B (S n)) (incA n) (incB n))
-          (fun n => fmap2 (A n) (A (S n)) (B n) (B (S n)) (incA n) (incB n))
-          (fmap2
-             (F:=F)
-             (G { n & A n} { n & B n}) { n & G (A n) (B n) }
-             (H { n & A n} { n & B n}) { n & H (A n) (B n) }
-             (fmapMax2 A B incA incB)
-             (fmapMax2 A B incA incB)
-             x)
-  |}.
-Next Obligation.
-  repeat intro.
-  apply fmap2Proper; [ apply fmap2Proper | apply fmap2Proper | ]; assumption.
-Defined.
-Next Obligation.
-  etransitivity; [ | apply fmap2Id ].
-  apply fmap2Proper; [ | | reflexivity ];
-    repeat intro; subst x; apply fmap2Id.
-Defined.
-Next Obligation.
-  repeat rewrite fmap2Comp.
-  apply fmap2Proper; [ | | reflexivity ];
-    repeat intro; subst x; apply fmap2Comp.
-Defined.
-Next Obligation.
-  etransitivity;
-    [ apply
-        (fmapMax2Eq (F:=F) _ _ _ _
-           (fun n => fmap2 (F:=G) (A n) (A (S n)) (B n) (B (S n)) (incA n) (incB n))
-           (fun n => fmap2 (F:=H) (A n) (A (S n)) (B n) (B (S n)) (incA n) (incB n))
-           (fun n => fmap2 (F:=G) (A n) C (B n) D (f n) (g n))
-           (fun n => fmap2 (F:=H) (A n) C (B n) D (f n) (g n)))
-    | ].
-  - intros. rewrite fmap2Comp.
-    apply fmap2Proper; [ | | reflexivity ];
-      repeat intro; subst x; [ apply H3 | apply H4 ].
-  - intros. rewrite fmap2Comp.
-    apply fmap2Proper; [ | | reflexivity ];
-      repeat intro; subst x; [ apply H3 | apply H4 ].
-  - rewrite fmap2Comp.
-    apply fmap2Proper; [ | | reflexivity ];
-      repeat intro; subst x; apply fmapMax2Eq; assumption.
-Defined.
-
-
-(** An inductive description of recursive function types and their arguments **)
-
-(* NOTE: lrt_u is really just entree_u + 1, but Coq doesn't like that in some
-places where we need to write it, so we just define it as a new universe *)
-Universe lrt_u.
-Constraint entree_u < lrt_u.
-
-(* An encoded argument type for a recursive function and its arguments *)
-Inductive LetRecType : Type@{lrt_u} :=
-(* These three constructors represent functions of 0 or more arguments *)
-| LRT_SpecM (R : LetRecType) : LetRecType
-| LRT_FunDep (A : Type@{entree_u}) (rest : A -> LetRecType) : LetRecType
-| LRT_FunClos (A : LetRecType) (rest : LetRecType) : LetRecType
-(* These constructors represent the argument types used in functions *)
-| LRT_Type (A : Type@{entree_u}) : LetRecType
-| LRT_BinOp F `{ColimFunctor2 F} (A B : LetRecType) : LetRecType
-| LRT_Sigma (A : Type@{entree_u}) (B : A -> LetRecType) : LetRecType
-.
-
-(* A FunStack is a list of LetRecTypes representing all of the functions bound
-   by multiFixS that are currently in scope *)
-Definition FunStack : Type@{lrt_u} := plist LetRecType.
-
-(* A trivially inhabited "default" LetRecType *)
-Definition default_lrt : LetRecType :=
-  LRT_FunDep Empty_set (fun _ => LRT_SpecM (LRT_Type Empty_set)).
-
-(* Get the nth element of a FunStack list, or Empty_set -> Empty_set if n is too big *)
-Definition nthLRT (stk : FunStack) n : LetRecType :=
-  nth_default' default_lrt stk n.
-
-Definition nthClos (Closs : plist (LetRecType -> Type@{entree_u})) n
-  : LetRecType -> Type@{entree_u} :=
-  nth_default' (A:=LetRecType -> Type@{entree_u}) (fun _ => Empty_set) Closs n.
-
-(* An argument to a recursive function call, which is a decoding of a LetRecType
-to its corresponding Coq type except that functions are interpreted using the
-supplied type functor *)
-Fixpoint LRTArgF (Clos : LetRecType -> Type@{entree_u}) (argTp : LetRecType)
-  : Type@{entree_u} :=
-  match argTp with
-  | LRT_SpecM R => Clos (LRT_SpecM R)
-  | LRT_FunDep A B => Clos (LRT_FunDep A B)
-  | LRT_FunClos A B => Clos (LRT_FunClos A B)
-  | LRT_Type A => A
-  | LRT_BinOp F A B => F (LRTArgF Clos A) (LRTArgF Clos B)
-  | LRT_Sigma A B => { x:A & LRTArgF Clos (B x) }
-  end.
-
-
-(**
- ** Sequences of N arguments
- **)
-
-(* The head input type of a monadic function type described by a LetRecType *)
-Definition LRTHead (Arg: LetRecType -> Type@{entree_u}) lrt : Type@{entree_u} :=
-  match lrt with
-  | LRT_SpecM R => Empty_set
-  | LRT_FunDep A B => A
-  | LRT_FunClos A B => Arg A
-  | LRT_Type A => Empty_set
-  | LRT_BinOp F A B => Empty_set
-  | LRT_Sigma A B => Empty_set
-  end.
-
-(* The dependent part of the LRTHead type *)
-Definition LRTDepHead lrt : Type@{entree_u} :=
-  match lrt with
-  | LRT_SpecM R => Empty_set
-  | LRT_FunDep A B => A
-  | LRT_FunClos A B => unit
-  | LRT_Type A => Empty_set
-  | LRT_BinOp F A B => Empty_set
-  | LRT_Sigma A B => Empty_set
-  end.
-
-(* The closure part of the LRTHead type *)
-Definition LRTClosHead (Arg: LetRecType -> Type@{entree_u}) lrt : Type@{entree_u} :=
-  match lrt with
-  | LRT_SpecM R => Empty_set
-  | LRT_FunDep A B => unit
-  | LRT_FunClos A B => Arg A
-  | LRT_Type A => Empty_set
-  | LRT_BinOp F A B => Empty_set
-  | LRT_Sigma A B => Empty_set
-  end.
-
-(* Project the dependent part of an LRTHead *)
-Definition projLRTHeadD Arg lrt : LRTHead Arg lrt -> LRTDepHead lrt :=
-  match lrt return LRTHead Arg lrt -> LRTDepHead lrt with
-  | LRT_SpecM R => fun bot => match bot with end
-  | LRT_FunDep A B => fun a => a
-  | LRT_FunClos A B => fun arg => tt
-  | LRT_Type A => fun bot => match bot with end
-  | LRT_BinOp F A B => fun bot => match bot with end
-  | LRT_Sigma A B => fun bot => match bot with end
-  end.
-
-(* Project the closure part of an LRTHead *)
-Definition projLRTHeadC Arg lrt : LRTHead Arg lrt -> LRTClosHead Arg lrt :=
-  match lrt return LRTHead Arg lrt -> LRTClosHead Arg lrt with
-  | LRT_SpecM R => fun bot => match bot with end
-  | LRT_FunDep A B => fun a => tt
-  | LRT_FunClos A B => fun arg => arg
-  | LRT_Type A => fun bot => match bot with end
-  | LRT_BinOp F A B => fun bot => match bot with end
-  | LRT_Sigma A B => fun bot => match bot with end
-  end.
-
-(* Given the dependent head argument of lrt, compute its tail LetRecType *)
-Definition LRTTail lrt : LRTDepHead lrt -> LetRecType :=
-  match lrt return LRTDepHead lrt -> LetRecType with
-  | LRT_SpecM R => fun bot => match bot with end
-  | LRT_FunDep A B => fun a => B a
-  | LRT_FunClos A B => fun _ => B
-  | LRT_Type A => fun bot => match bot with end
-  | LRT_BinOp F A B => fun bot => match bot with end
-  | LRT_Sigma A B => fun bot => match bot with end
-  end.
-
-Fixpoint LRTDepArgsAndRet n lrt : { T:Type@{entree_u} & T -> LetRecType } :=
-  match n with
-  | 0 => existT (fun T => T -> LetRecType) unit (fun _ => lrt)
-  | S n' =>
-      existT (fun T => T -> LetRecType)
-        { args: projT1 (LRTDepArgsAndRet n' lrt) &
-                  LRTDepHead (projT2 (LRTDepArgsAndRet n' lrt) args) }
-             (fun args =>
-                LRTTail (projT2 (LRTDepArgsAndRet n' lrt) (projT1 args)) (projT2 args))
-  end.
-
-Definition LRTDepArgs n lrt : Type@{entree_u} := projT1 (LRTDepArgsAndRet n lrt).
-
-Definition LRTDepArgsOut n lrt (args: LRTDepArgs n lrt) : LetRecType :=
-  projT2 (LRTDepArgsAndRet n lrt) args.
-
-Definition LRTDepArgsNil lrt : LRTDepArgs 0 lrt := tt.
-
-Definition LRTDepArgsConsR n lrt (dargs: LRTDepArgs n lrt)
-  (darg: LRTDepHead (LRTDepArgsOut n lrt dargs)) : LRTDepArgs (S n) lrt :=
-  existT _ dargs darg.
-
-Definition LRTDepArgsConsROutEq n lrt dargs darg :
-  LRTDepArgsOut (S n) lrt (LRTDepArgsConsR n lrt dargs darg) =
-    LRTTail (LRTDepArgsOut n lrt dargs) darg :=
-  eq_refl _. (* Checks that this holds by definitional equality *)
-
-Fixpoint LRTClosArgsF (Arg: LetRecType -> Type@{entree_u}) n lrt
-  : LRTDepArgs n lrt -> Type@{entree_u} :=
-  match n return LRTDepArgs n lrt -> Type@{entree_u} with
-  | 0 => fun _ => unit
-  | S n' =>
-      fun dargs =>
-        prod (LRTClosArgsF Arg n' lrt (projT1 dargs))
-          (LRTClosHead Arg (LRTDepArgsOut n' lrt (projT1 dargs)))
-  end.
-
-Definition LRTClosArgsFNil Arg lrt : LRTClosArgsF Arg 0 lrt (LRTDepArgsNil lrt) := tt.
-
-Definition LRTClosArgsFConsR Arg n lrt dargs (cargs: LRTClosArgsF Arg n lrt dargs)
-  (darg: LRTDepHead (LRTDepArgsOut n lrt dargs))
-  (carg: LRTClosHead Arg (LRTDepArgsOut n lrt dargs)) :
-  LRTClosArgsF Arg (S n) lrt (LRTDepArgsConsR n lrt dargs darg) :=
-  (cargs, carg).
-
-Definition LRTArgsF Arg n lrt : Type@{entree_u} :=
-  { dep_args:LRTDepArgs n lrt & LRTClosArgsF Arg n lrt dep_args }.
-
-Definition LRTArgsFOut Arg n lrt : LRTArgsF Arg n lrt -> LetRecType :=
-  fun args => LRTDepArgsOut n lrt (projT1 args).
-
-Definition LRTArgsFNil Arg lrt : LRTArgsF Arg 0 lrt := existT _ tt tt.
-
-Definition LRTArgsFConsR Arg n lrt (args: LRTArgsF Arg n lrt)
-  (darg: LRTDepHead (LRTDepArgsOut n lrt (projT1 args)))
-  (carg: LRTClosHead Arg (LRTDepArgsOut n lrt (projT1 args))) :
-  LRTArgsF Arg (S n) lrt :=
-  existT _ (LRTDepArgsConsR n lrt (projT1 args) darg)
-    (LRTClosArgsFConsR Arg n lrt (projT1 args) (projT2 args) darg carg).
-
-Definition LRTArgsFConsROutEq Arg n lrt args darg carg :
-  LRTArgsFOut Arg (S n) lrt (LRTArgsFConsR Arg n lrt args darg carg) =
-    LRTTail (LRTArgsFOut Arg n lrt args) darg :=
-  eq_refl _. (* Checks that this holds by definitional equality *)
-
-
-(**
- ** Defining closures
- **)
-
-Definition ClosElemF (Closs : plist (LetRecType -> Type@{entree_u})) lrt
-  : Type@{entree_u} :=
-  { n & nthClos Closs n lrt }.
-
-Definition ClosElemFConsClos Clos Closs lrt (ce: ClosElemF Closs lrt)
-  : ClosElemF (pcons Clos Closs) lrt :=
-  existT _ (S (projT1 ce)) (projT2 ce).
-
-Record LRTClosF stk (Closs : plist (LetRecType -> Type@{entree_u})) lrt
-  : Type@{entree_u} :=
-  { lrtClosNum : nat;
-    lrtClosNumArgs : nat;
-    lrtClosDepArgs : LRTDepArgs lrtClosNumArgs (nthLRT stk lrtClosNum);
-    lrtClosClosArgs : LRTClosArgsF (LRTArgF (ClosElemF Closs)) lrtClosNumArgs
-                        (nthLRT stk lrtClosNum) lrtClosDepArgs;
-    lrtClosLRTEq : LRTDepArgsOut lrtClosNumArgs _ lrtClosDepArgs = lrt }.
-
-Definition LRTClosFOut {stk Closs lrt} (clos: LRTClosF stk Closs lrt) : LetRecType :=
-  LRTDepArgsOut (lrtClosNumArgs _ _ _ clos) _ (lrtClosDepArgs _ _ _ clos).
-
-Definition applyLRTClosFRaw stk Closs lrt (clos: LRTClosF stk Closs lrt)
-  (darg: LRTDepHead (LRTClosFOut clos))
-  (carg: LRTClosHead (LRTArgF (ClosElemF Closs)) (LRTClosFOut clos))
-  : LRTClosF stk Closs (LRTTail (LRTClosFOut clos) darg) :=
-  {|
-    lrtClosNum := lrtClosNum _ _ _ clos;
-    lrtClosNumArgs := S (lrtClosNumArgs _ _ _ clos);
-    lrtClosDepArgs := LRTDepArgsConsR _ _ (lrtClosDepArgs _ _ _ clos) darg;
-    lrtClosClosArgs := LRTClosArgsFConsR _ _ _ _ (lrtClosClosArgs _ _ _ clos) darg carg;
-    lrtClosLRTEq := eq_refl _;
-  |}.
-
-Program Definition applyLRTClosF stk Closs lrt (clos: LRTClosF stk Closs lrt) :
-  forall darg: LRTDepHead lrt, LRTClosHead (LRTArgF (ClosElemF Closs)) lrt ->
-                               LRTClosF stk Closs (LRTTail lrt darg) :=
-  eq_rect
-    (LRTClosFOut clos)
-    (fun lrt' => forall darg, LRTClosHead (LRTArgF (ClosElemF Closs)) lrt' ->
-                              LRTClosF stk Closs (LRTTail lrt' darg))
-    (applyLRTClosFRaw stk Closs lrt clos)
-    lrt (lrtClosLRTEq _ _ _ clos).
-
-
-(**
- ** Lifting functions for closures and arguments
- **)
-
-Fixpoint LRTArgFConsClos Clos Closs argTp
-  : LRTArgF (ClosElemF Closs) argTp ->
-    LRTArgF (ClosElemF (pcons Clos Closs)) argTp :=
-  match argTp return LRTArgF (ClosElemF Closs) argTp ->
-                     LRTArgF (ClosElemF (pcons Clos Closs)) argTp with
-  | LRT_SpecM R => ClosElemFConsClos Clos Closs _
-  | LRT_FunDep A B => ClosElemFConsClos Clos Closs _
-  | LRT_FunClos A B => ClosElemFConsClos Clos Closs _
-  | LRT_Type A => fun a => a
-  | LRT_BinOp F A B =>
-      fmap2 _ _ _ _ (LRTArgFConsClos Clos Closs A) (LRTArgFConsClos Clos Closs B)
-  | LRT_Sigma A B =>
-      fun p => existT _ (projT1 p)
-                 (LRTArgFConsClos Clos Closs (B (projT1 p)) (projT2 p))
-  end.
-
-Definition LRTClosHeadConsClos Clos Closs lrt
-  : LRTClosHead (LRTArgF (ClosElemF Closs)) lrt ->
-    LRTClosHead (LRTArgF (ClosElemF (pcons Clos Closs))) lrt :=
-  match lrt return LRTClosHead (LRTArgF (ClosElemF Closs)) lrt ->
-                   LRTClosHead (LRTArgF (ClosElemF (pcons Clos Closs))) lrt with
-  | LRT_SpecM R => fun bot => match bot with end
-  | LRT_FunDep A B => fun u => u
-  | LRT_FunClos A B => fun arg => LRTArgFConsClos Clos Closs A arg
-  | LRT_Type A => fun bot => match bot with end
-  | LRT_BinOp F A B => fun bot => match bot with end
-  | LRT_Sigma A B => fun bot => match bot with end
-  end.
-
-Fixpoint LRTClosArgsFConsClos Clos Closs n lrt :
-  forall dargs, LRTClosArgsF (LRTArgF (ClosElemF Closs)) n lrt dargs ->
-                LRTClosArgsF (LRTArgF (ClosElemF (pcons Clos Closs))) n lrt dargs :=
-  match n return
-        forall dargs,
-          LRTClosArgsF (LRTArgF (ClosElemF Closs)) n lrt dargs ->
-          LRTClosArgsF (LRTArgF (ClosElemF (pcons Clos Closs))) n lrt dargs
-  with
-  | 0 => fun _ u => u
-  | S n' =>
-      fun dargs cargs =>
-        (LRTClosArgsFConsClos Clos Closs n' lrt (projT1 dargs) (fst cargs),
-          LRTClosHeadConsClos Clos Closs _ (snd cargs))
-  end.
-
-Definition LRTClosFConsClos stk Clos Closs lrt
-  (clos : LRTClosF stk Closs lrt) : LRTClosF stk (pcons Clos Closs) lrt :=
-  {|
-    lrtClosNum := lrtClosNum _ _ _ clos;
-    lrtClosNumArgs := lrtClosNumArgs _ _ _ clos;
-    lrtClosDepArgs := lrtClosDepArgs _ _ _ clos;
-    lrtClosClosArgs :=
-      LRTClosArgsFConsClos Clos Closs _ _ _ (lrtClosClosArgs _ _ _ clos);
-    lrtClosLRTEq := lrtClosLRTEq _ _ _ clos;
- |}.
-
-
-(**
- ** Tie the knot by defining closures by level
- **)
-
-Fixpoint LRTClosTypes stk lvl : plist (LetRecType -> Type@{entree_u}) :=
-  match lvl with
-  | 0 => pnil
-  | S lvl' =>
-      pcons (LRTClosF stk (LRTClosTypes stk lvl')) (LRTClosTypes stk lvl')
-  end.
-
-Definition ClosElemLvl stk lvl lrt : Type@{entree_u} :=
-  ClosElemF (LRTClosTypes stk lvl) lrt.
-
-Definition ClosElemLvlInc stk lvl lrt (clos: ClosElemLvl stk lvl lrt)
-  : ClosElemLvl stk (S lvl) lrt :=
-  ClosElemFConsClos _ _ lrt clos.
-
-Definition LRTArgLvl stk argTp lvl : Type@{entree_u} :=
-  LRTArgF (ClosElemLvl stk lvl) argTp.
-
-Definition LRTArgLvlInc stk argTp lvl (arg: LRTArgLvl stk argTp lvl)
-  : LRTArgLvl stk argTp (S lvl) :=
-  LRTArgFConsClos _ _ argTp arg.
-
-Definition LRTArgHeadLvl stk lrt lvl : Type@{entree_u} :=
-  LRTClosHead (fun argTp => LRTArgLvl stk argTp lvl) lrt.
-
-Definition LRTArgHeadLvlInc stk lrt lvl (arg: LRTArgHeadLvl stk lrt lvl) :
-  LRTArgHeadLvl stk lrt (S lvl) :=
-  LRTClosHeadConsClos _ _ lrt arg.
-
-Definition LRTClosArgsLvl stk n lrt lvl dargs :=
-  LRTClosArgsF (fun argTp => LRTArgLvl stk argTp lvl) n lrt dargs.
-
-Definition LRTClosArgsLvlInc stk n lrt lvl dargs
-  (cargs: LRTClosArgsLvl stk n lrt lvl dargs)
-  : LRTClosArgsLvl stk n lrt (S lvl) dargs :=
-  LRTClosArgsFConsClos _ _ n lrt dargs cargs.
-
-Definition LRTClosLvl stk lrt lvl :=
-  LRTClosF stk (LRTClosTypes stk lvl) lrt.
-
-Definition LRTClosLvlInc stk lrt lvl (clos: LRTClosLvl stk lrt lvl)
-  : LRTClosLvl stk lrt (S lvl) :=
-  LRTClosFConsClos stk _ _ lrt clos.
-
-Definition applyLRTClosLvl stk lrt lvl (clos: LRTClosLvl stk lrt lvl)
-  (darg: LRTDepHead lrt) (carg: LRTArgHeadLvl stk lrt lvl)
-  : LRTClosLvl stk (LRTTail lrt darg) lvl :=
-  applyLRTClosF stk _ lrt clos darg carg.
-
-
-(**
- ** Defining closures and arguments at arbitrary levels, and mapping them to and
- ** from their corresponding leveled types
- **)
-
-Definition LRTClos stk lrt : Type@{entree_u} :=
-  { lvl & LRTClosLvl stk lrt lvl }.
-
-Definition LRTClosToClosElem stk lrt (clos: LRTClos stk lrt)
-  : { lvl & ClosElemLvl stk lvl lrt } :=
-  existT _ (S (projT1 clos)) (existT _ 0 (projT2 clos)).
-
-Fixpoint LRTClosFromClosElemH stk lrt lvl lft :
-  nthClos (LRTClosTypes stk lvl) lft lrt -> LRTClosLvl stk lrt (lvl - S lft) :=
-  match lvl return nthClos (LRTClosTypes stk lvl) lft lrt ->
-                   LRTClosLvl stk lrt (lvl - S lft) with
-  | 0 => fun bot => match bot with end
-  | S lvl' =>
-      match lft return nthClos (LRTClosTypes stk (S lvl')) lft lrt ->
-                       LRTClosLvl stk lrt (lvl' - lft) with
-      | 0 =>
-          match lvl' return nthClos (LRTClosTypes stk (S lvl')) 0 lrt ->
-                            LRTClosLvl stk lrt (lvl' - 0) with
-          | 0 => fun clos => clos
-          | S lvl'' => fun clos => clos
-          end
-      | S lft' => fun clos => LRTClosFromClosElemH stk lrt lvl' lft' clos
-      end
-  end.
-
-Definition LRTClosFromClosElem stk lrt lvl
-  (clos: ClosElemLvl stk lvl lrt) : LRTClos stk lrt :=
-  existT _ _ (LRTClosFromClosElemH stk lrt lvl (projT1 clos) (projT2 clos)).
-
-Definition LRTClosFromClosElemInc stk lrt lvl clos :
-  LRTClosFromClosElem stk lrt (S lvl) (ClosElemLvlInc stk lvl lrt clos) =
-  LRTClosFromClosElem stk lrt lvl clos :=
-  eq_refl _. (* Check that this equality holds by definitional equality *)
-
-Lemma LRTClosToFromClosElem stk lrt clos :
-  LRTClosFromClosElem stk lrt
-    (projT1 (LRTClosToClosElem stk lrt clos))
-    (projT2 (LRTClosToClosElem stk lrt clos)) = clos.
-Proof.
-  destruct clos as [lvl clos]. revert clos; induction lvl; intros; reflexivity.
-Qed.
-
-Definition LRTArg stk argTp : Type@{entree_u} := LRTArgF (LRTClos stk) argTp.
-
-Fixpoint LRTArgMax stk argTp
-  : LRTArg stk argTp -> { lvl & LRTArgLvl stk argTp lvl } :=
-  match argTp return LRTArg stk argTp -> { lvl & LRTArgLvl stk argTp lvl } with
-  | LRT_SpecM R => fun clos => LRTClosToClosElem stk _ clos
-  | LRT_FunDep A B => fun clos => LRTClosToClosElem stk _ clos
-  | LRT_FunClos A B => fun clos => LRTClosToClosElem stk _ clos
-  | LRT_Type A => fun a => existT _ 0 a
-  | LRT_BinOp F A B =>
-      fun x =>
-        fmapMax2 (LRTArgLvl stk A) (LRTArgLvl stk B)
-          (LRTArgLvlInc stk A) (LRTArgLvlInc stk B)
-          (fmap2 _ _ _ _ (LRTArgMax stk A) (LRTArgMax stk B) x)
-  | LRT_Sigma A B =>
-      fun p =>
-        existT _ (projT1 (LRTArgMax stk (B (projT1 p)) (projT2 p)))
-          (existT _ (projT1 p) (projT2 (LRTArgMax stk (B (projT1 p)) (projT2 p))))
-  end.
-
-
-Fixpoint LRTArgMaxInv stk argTp lvl :
-  LRTArgLvl stk argTp lvl -> LRTArg stk argTp :=
-  match argTp return LRTArgLvl stk argTp lvl -> LRTArg stk argTp with
-  | LRT_SpecM R => fun clos => LRTClosFromClosElem stk _ _ clos
-  | LRT_FunDep A B => fun clos => LRTClosFromClosElem stk _ _ clos
-  | LRT_FunClos A B => fun clos => LRTClosFromClosElem stk _ _ clos
-  | LRT_Type A => fun a => a
-  | LRT_BinOp F A B =>
-      fmap2
-        (LRTArgLvl stk A lvl) (LRTArg stk A) (LRTArgLvl stk B lvl) (LRTArg stk B)
-        (LRTArgMaxInv stk A lvl) (LRTArgMaxInv stk B lvl)
-  | LRT_Sigma A B =>
-      fun p =>
-        existT _ (projT1 p) (LRTArgMaxInv stk (B (projT1 p)) lvl (projT2 p))
-  end.
-
-Lemma LRTArgMaxInvInc stk argTp lvl (arg : LRTArgLvl stk argTp lvl) :
-  LRTArgMaxInv stk argTp lvl arg
-  = LRTArgMaxInv stk argTp (S lvl) (LRTArgLvlInc stk argTp lvl arg).
-Proof.
-  revert arg; induction argTp; intros; simpl; try reflexivity.
-  - unfold LRTArgLvlInc; simpl.
-    rewrite fmap2Comp.
-    apply (fmap2Proper (F:=F)); [ | | reflexivity ];
-      repeat intro; subst x; [ apply IHargTp1 | apply IHargTp2 ].
-  - f_equal; apply H.
-Qed.
-
-Lemma LRTArgMaxInvEq stk argTp arg :
-  LRTArgMaxInv stk argTp (projT1 (LRTArgMax stk argTp arg))
-    (projT2 (LRTArgMax stk argTp arg))
-  = arg.
-Proof.
-  revert arg; induction argTp; intros; simpl.
-  - apply LRTClosToFromClosElem.
-  - apply LRTClosToFromClosElem.
-  - apply LRTClosToFromClosElem.
-  - reflexivity.
-  - etransitivity; [ apply (fmapMax2Eq (F:=F)) | ].
-    + apply LRTArgMaxInvInc.
-    + apply LRTArgMaxInvInc.
-    + rewrite fmap2Comp.
-      etransitivity; [ | apply (fmap2Id (F:=F)) ].
-      apply (fmap2Proper (F:=F)); [ | | reflexivity ];
-        repeat intro; subst x; [ apply IHargTp1 | apply IHargTp2 ].
-  - destruct arg. simpl. rewrite H. reflexivity.
-Qed.
-
-
-Definition LRTArgHead stk lrt := LRTClosHead (LRTArg stk) lrt.
-
-Definition LRTArgHeadMax stk lrt :
-  LRTArgHead stk lrt -> { lvl & LRTArgHeadLvl stk lrt lvl } :=
-  match lrt return LRTArgHead stk lrt -> { lvl & LRTArgHeadLvl stk lrt lvl } with
-  | LRT_SpecM R => fun bot => match bot with end
-  | LRT_FunDep A B => fun u => existT _ 0 u
-  | LRT_FunClos A B => fun arg => LRTArgMax stk _ arg
-  | LRT_Type A => fun bot => match bot with end
-  | LRT_BinOp F A B => fun bot => match bot with end
-  | LRT_Sigma A B => fun bot => match bot with end
-  end.
-
-Definition LRTArgHeadMaxInv stk lrt lvl :
-  LRTArgHeadLvl stk lrt lvl -> LRTArgHead stk lrt :=
-  match lrt return LRTArgHeadLvl stk lrt lvl -> LRTArgHead stk lrt with
-  | LRT_SpecM R => fun bot => match bot with end
-  | LRT_FunDep A B => fun u => u
-  | LRT_FunClos A B => fun arg => LRTArgMaxInv stk A lvl arg
-  | LRT_Type A => fun bot => match bot with end
-  | LRT_BinOp F A B => fun bot => match bot with end
-  | LRT_Sigma A B => fun bot => match bot with end
-  end.
-
-Lemma LRTArgHeadMaxInvInc stk lrt lvl (arg : LRTArgHeadLvl stk lrt lvl) :
-  LRTArgHeadMaxInv stk lrt lvl arg
-  = LRTArgHeadMaxInv stk lrt (S lvl) (LRTArgHeadLvlInc stk lrt lvl arg).
-Proof.
-  destruct lrt; try reflexivity; try destruct arg.
-  apply LRTArgMaxInvInc.
-Qed.
-
-Lemma LRTArgHeadMaxInvEq stk lrt arg :
-  LRTArgHeadMaxInv stk lrt (projT1 (LRTArgHeadMax stk lrt arg))
-    (projT2 (LRTArgHeadMax stk lrt arg))
-  = arg.
-Proof.
-  revert arg; destruct lrt; intros; simpl; try reflexivity; try destruct arg.
-  apply LRTArgMaxInvEq.
-Qed.
-
-
-Definition LRTClosArgs stk n lrt dargs : Type@{entree_u} :=
-  LRTClosArgsF (LRTArgF (LRTClos stk)) n lrt dargs.
-
-Fixpoint LRTClosArgsMax stk n lrt :
-  forall dargs, LRTClosArgs stk n lrt dargs ->
-                { lvl & LRTClosArgsLvl stk n lrt lvl dargs } :=
-  match n return forall dargs, LRTClosArgs stk n lrt dargs ->
-                               { lvl & LRTClosArgsLvl stk n lrt lvl dargs } with
-  | 0 => fun _ u => existT _ 0 u
-  | S n' =>
-      fun dargs cargs =>
-        levelCombine
-          (fun lvl => LRTClosArgsLvl stk n' lrt lvl (projT1 dargs))
-          (fun lvl => LRTArgHeadLvl stk _ lvl)
-          (fun lvl => LRTClosArgsLvl stk (S n') lrt lvl dargs)
-          (fun lvl => LRTClosArgsLvlInc stk n' _ lvl (projT1 dargs))
-          (fun lvl => LRTArgHeadLvlInc stk _ lvl)
-          (fun n a b => (a, b))
-          (LRTClosArgsMax stk n' lrt (projT1 dargs) (fst cargs))
-          (LRTArgHeadMax stk _ (snd cargs))
-  end.
-
-Fixpoint LRTClosArgsMaxInv stk n lrt lvl :
-  forall dargs, LRTClosArgsLvl stk n lrt lvl dargs ->
-                LRTClosArgs stk n lrt dargs :=
-  match n return forall dargs, LRTClosArgsLvl stk n lrt lvl dargs ->
-                               LRTClosArgs stk n lrt dargs with
-  | 0 => fun _ u => u
-  | S n' =>
-      fun dargs cargs =>
-        (LRTClosArgsMaxInv stk n' lrt lvl (projT1 dargs) (fst cargs),
-          LRTArgHeadMaxInv stk _ lvl (snd cargs))
-  end.
-
-Lemma LRTClosArgsMaxInvInc stk n lrt lvl dargs cargs :
-  LRTClosArgsMaxInv stk n lrt lvl dargs cargs
-  = LRTClosArgsMaxInv stk n lrt (S lvl) dargs
-      (LRTClosArgsLvlInc stk n lrt lvl dargs cargs).
-Proof.
-  revert lrt dargs cargs; induction n; intros.
-  - reflexivity.
-  - simpl. f_equal; [ apply IHn | apply LRTArgHeadMaxInvInc ].
-Qed.
-
-Lemma LRTClosArgsMaxInvEq stk n lrt dargs cargs :
-  LRTClosArgsMaxInv stk n lrt
-    (projT1 (LRTClosArgsMax stk n lrt dargs cargs))
-    dargs
-    (projT2 (LRTClosArgsMax stk n lrt dargs cargs)) =
-    cargs.
-Proof.
-  revert lrt dargs cargs; induction n; intros.
-  - reflexivity.
-  - destruct cargs. simpl. f_equal.
-    + rewrite (elimLevelMaxR _ _ _ _ _
-                 (fun lvl cargs =>
-                    LRTClosArgsMaxInv stk n _ lvl (projT1 dargs) cargs));
-        [ apply IHn | intros; apply LRTClosArgsMaxInvInc ].
-    + rewrite elimLevelMaxL;
-        [ apply LRTArgHeadMaxInvEq | intros; apply LRTArgHeadMaxInvInc ].
-Qed.
-
-
-Definition applyLRTClos stk lrt (clos: LRTClos stk lrt)
-  (darg: LRTDepHead lrt) (carg: LRTArgHead stk lrt)
-  : LRTClos stk (LRTTail lrt darg) :=
-  levelCombine
-    (LRTClosLvl stk lrt)
-    (LRTArgHeadLvl stk lrt)
-    (LRTClosLvl stk (LRTTail lrt darg))
-    (LRTClosLvlInc stk lrt)
-    (LRTArgHeadLvlInc stk lrt)
-    (fun lvl clos' carg' => applyLRTClosLvl stk lrt lvl clos' darg carg')
-    clos
-    (LRTArgHeadMax stk lrt carg).
-
-Definition applyLRTClosDep stk A B (clos: LRTClos stk (LRT_FunDep A B)) (a:A)
-  : LRTClos stk (B a) := applyLRTClos stk (LRT_FunDep A B) clos a tt.
-
-Definition applyLRTClosClos stk A B (clos: LRTClos stk (LRT_FunClos A B))
-  (arg: LRTArg stk A) : LRTClos stk B := applyLRTClos stk (LRT_FunClos A B) clos tt arg.
-
-Fixpoint applyLRTClosNRet stk n lrt : Type@{entree_u} :=
-  match n with
-  | 0 => LRTClos stk lrt
-  | S n' =>
-      match lrt with
-      | LRT_SpecM R => Empty_set -> Empty_set
-      | LRT_FunDep A B => forall a:A, applyLRTClosNRet stk n' (B a)
-      | LRT_FunClos A B => LRTArg stk A -> applyLRTClosNRet stk n' B
-      | LRT_Type A => Empty_set -> Empty_set
-      | LRT_BinOp F A B => Empty_set -> Empty_set
-      | LRT_Sigma A B => Empty_set -> Empty_set
-      end
-  end.
-
-Fixpoint applyLRTClosN stk n lrt : LRTClos stk lrt -> applyLRTClosNRet stk n lrt :=
-  match n return LRTClos stk lrt -> applyLRTClosNRet stk n lrt with
-  | 0 => fun clos => clos
-  | S n' =>
-      match lrt return LRTClos stk lrt -> applyLRTClosNRet stk (S n') lrt with
-      | LRT_SpecM R => fun _ bot => bot
-      | LRT_FunDep A B => fun clos a =>
-                            applyLRTClosN stk n' (B a) (applyLRTClosDep stk A B clos a)
-      | LRT_FunClos A B => fun clos arg =>
-                             applyLRTClosN stk n' B (applyLRTClosClos stk A B clos arg)
-      | LRT_Type A => fun _ bot => bot
-      | LRT_BinOp F A B => fun _ bot => bot
-      | LRT_Sigma A B => fun _ bot => bot
-      end
-  end.
-
-
-(**
- ** Complete lists of input arguments to corecursive functions
- **)
-
-(* A dependent tuple type of all the inputs of a LetRecType, i.e., return the
-   type { x:A & { y:B & ... { z:C & unit } ...}} from a LetRecType that
-   represents forall a b c..., SpecM ... (R a b c ...). A LetRectype that is not
-   a function type just becomes the Empty_set type. *)
-Fixpoint LRTInput stack lrt : Type@{entree_u} :=
-  match lrt with
-  | LRT_SpecM _ => unit
-  | LRT_FunDep A rest => {a : A & LRTInput stack (rest a) }
-  | LRT_FunClos A rest => LRTArg stack A * LRTInput stack rest
-  | _ => Empty_set
-  end.
-
-(* The output type (R a b c ...) of a LetRecType that represents the function
-   type forall a b c..., SpecM ... (R a b c ...) given a dependent tuple of
-   arguments to a function of that type *)
-Fixpoint LRTOutput stack lrt : EncodingType (LRTInput stack lrt) :=
-  match lrt with
-  | LRT_SpecM R => fun _ => LRTArg stack R
-  | LRT_FunDep A rest => fun args =>
-                           let '(existT _ a args') := args in
-                           LRTOutput stack (rest a) args'
-  | LRT_FunClos A rest => fun args => LRTOutput stack rest (snd args)
-  | _ => fun args => match args with end
-  end.
-
-
-Definition LRTInputCons stk lrt :
-  forall darg:LRTDepHead lrt, LRTClosHead (LRTArgF (LRTClos stk)) lrt ->
-                              LRTInput stk (LRTTail lrt darg) ->
-                              LRTInput stk lrt :=
-  match lrt return forall darg, LRTClosHead (LRTArgF (LRTClos stk)) lrt ->
-                                LRTInput stk (LRTTail lrt darg) ->
-                                LRTInput stk lrt with
-  | LRT_SpecM R => fun bot => match bot with end
-  | LRT_FunDep A B => fun a _ inps => existT _ a inps
-  | LRT_FunClos A B => fun _ arg inps => (arg, inps)
-  | LRT_Type A => fun bot => match bot with end
-  | LRT_BinOp F A B => fun bot => match bot with end
-  | LRT_Sigma A B => fun bot => match bot with end
-  end.
-
-Lemma LRTInputConsOut stk lrt darg carg inps :
-  LRTOutput stk lrt (LRTInputCons stk lrt darg carg inps) =
-    LRTOutput stk _ inps.
-Proof.
-  destruct lrt; try destruct darg; reflexivity.
-Qed.
-
-Fixpoint LRTArgsToInput stk n lrt :
-  forall dargs, LRTClosArgs stk n lrt dargs ->
-                LRTInput stk (LRTDepArgsOut n lrt dargs) -> LRTInput stk lrt :=
-  match n return forall dargs, LRTClosArgs stk n lrt dargs ->
-                               LRTInput stk (LRTDepArgsOut n lrt dargs) ->
-                               LRTInput stk lrt
-  with
-  | 0 => fun _ _ inps => inps
-  | S n' =>
-      fun dargs cargs inps =>
-        LRTArgsToInput stk n' _ (projT1 dargs) (fst cargs)
-          (LRTInputCons stk _ (projT2 dargs) (snd cargs) inps)
-  end.
-
-Lemma LRTArgsToInputOut stk n lrt dargs cargs inps :
-  LRTOutput stk lrt (LRTArgsToInput stk n lrt dargs cargs inps) =
-    LRTOutput stk _ inps.
-Proof.
-  revert dargs cargs inps; induction n; [ reflexivity | ]; intros.
-  etransitivity; [ apply IHn | apply LRTInputConsOut ].
-Qed.
-
-
-(**
- ** N-ary functions over LetRecTypes
- **)
-
-(* Build the type forall a b c ..., F (a, (b, (c, ...))) for an arbitrary type
-   function F over an LRTInput. A LetRecType that is not a function type turns
-   into a function from v:Empty_set to F v *)
-Fixpoint lrtPi stack lrt : (LRTInput stack lrt -> Type) -> Type :=
-  match lrt return (LRTInput stack lrt -> Type) -> Type with
-  | LRT_SpecM _ => fun F => F tt
-  | LRT_FunDep A lrtF =>
-      fun F => forall a, lrtPi stack (lrtF a) (fun args => F (existT _ a args))
-  | LRT_FunClos A lrt' =>
-      fun F => forall a, lrtPi stack lrt' (fun args => F (a, args))
-  | _ => fun F => forall v:Empty_set, F v
-  end.
-
-(* Build an lrtPi function from a unary function on an LRTInput *)
-Fixpoint lrtLambda stack lrt
-  : forall (F : LRTInput stack lrt -> Type),
-    (forall args, F args) -> lrtPi stack lrt F :=
-  match lrt return
-        forall (F : LRTInput stack lrt -> Type),
-          (forall args, F args) -> lrtPi stack lrt F
-  with
-  | LRT_SpecM _ => fun _ f => f tt
-  | LRT_FunDep A lrtF =>
-    fun F f a => lrtLambda stack (lrtF a)
-                   (fun args => F (existT _ a args))
-                   (fun args => f (existT _ a args))
-  | LRT_FunClos A lrt' =>
-      fun F f a => lrtLambda stack lrt'
-                     (fun args => F (a, args))
-                     (fun args => f (a, args))
-  | _ => fun _ _ v => match v with end
-  end.
-
-(* Apply an lrtPi function *)
-Fixpoint lrtApply stack lrt
-  : forall F, lrtPi stack lrt F -> forall args, F args :=
-  match lrt return forall F, lrtPi stack lrt F -> forall args, F args with
-  | LRT_SpecM _ =>
-    fun F f u => match u return F u with | tt => f end
-  | LRT_FunDep A lrtF =>
-    fun F f args =>
-      match args return F args with
-      | existT _ arg args' =>
-        lrtApply stack (lrtF arg) (fun args' => F (existT _ arg args')) (f arg) args'
-      end
-  | LRT_FunClos A lrt' =>
-    fun F f args =>
-      match args return F args with
-      | (arg, args') =>
-        lrtApply stack lrt' (fun args' => F (arg, args')) (f arg) args'
-      end
-  | _ =>
-      fun _ _ v => match v with end
-  end.
-
-
-(**
- ** Calls to an arbitrary corecursive function in the stack
- **)
-
-(* A recursive call to one of the functions in a FunStack, specified by a
-natural number n that picks a specific index in the FunStack along with a set of
-arguments for that recursive call, relative to a given stack *)
-Inductive StackCall stack : Type@{entree_u} :=
-| StackCallOfArgs n (args : LRTInput stack (nthLRT stack n)).
-
-(* The return type for a StackCall recursive call, using a specific M *)
-Definition StackCallRet stack (args: StackCall stack) : Type@{entree_u} :=
-  match args with
-  | StackCallOfArgs _ n args => LRTOutput stack (nthLRT stack n) args
-  end.
-
-Definition LRTClosToCall stk R (clos: LRTClos stk (LRT_SpecM R)) : StackCall stk :=
-  StackCallOfArgs stk (lrtClosNum _ _ _ (projT2 clos))
-    (LRTArgsToInput stk
-       (lrtClosNumArgs _ _ _ (projT2 clos))
-       (nthLRT stk (lrtClosNum _ _ _ (projT2 clos)))
-       (lrtClosDepArgs _ _ _ (projT2 clos))
-       (LRTClosArgsMaxInv _ _ _ _ _ (lrtClosClosArgs _ _ _ (projT2 clos)))
-       (eq_rect (LRT_SpecM R) (LRTInput stk) tt _ (eq_sym (lrtClosLRTEq _ _ _ (projT2 clos))))).
-
-Lemma castLRTOutput stk lrt1 lrt2 (inps: LRTInput stk lrt2) (e: lrt1 = lrt2) :
-  LRTOutput stk lrt1 (eq_rect lrt2 (LRTInput stk) inps lrt1 (eq_sym e)) = LRTOutput stk lrt2 inps.
-Proof.
-  destruct e. reflexivity.
-Qed.
-
-Lemma LRTClosToCallRet stk R clos :
-  StackCallRet stk (LRTClosToCall stk R clos) = LRTArg stk R.
-Proof.
-  simpl. rewrite LRTArgsToInputOut. apply castLRTOutput.
-Qed.
-
 
 (**
  ** EncodingType and ReSum instances for defining SpecM
  **)
-
-Global Instance EncodingType_StackCall stack : EncodingType (StackCall stack) :=
-  StackCallRet stack.
 
 (* The error event type *)
 Inductive ErrorE : Set :=
@@ -1235,71 +46,28 @@ Inductive ErrorE : Set :=
 
 Global Instance EncodingType_ErrorE : EncodingType ErrorE := fun _ => Empty_set.
 
-(* Create an event type for either an event in E or a recursive call in a stack
-   Γ of recursive functions in scope *)
-Definition FunStackE (E : EvType@{entree_u}) (stack : FunStack) : Type@{entree_u} :=
-  StackCall stack + (ErrorE + E).
+(* The event type for SpecM computations, given an underlying event type *)
+Definition SpecE (E : EvType@{entree_u}) : Type@{entree_u} :=
+  SpecEvent (ErrorE + E).
 
-(* The return type for a FunStackE effect in a SpecM computation *)
-Definition FunStackERet E stack (e:FunStackE E stack) : Type@{entree_u} :=
-  encodes e.
+(* The return type for a SpecEE effect in a SpecM computation *)
+Definition SpecERet E (e:SpecE E) : Type@{entree_u} := encodes e.
 
-Global Instance EncodingType_FunStackE E stack : EncodingType (FunStackE E stack) :=
-  FunStackERet E stack.
+Definition SpecEv E : EvType := Build_EvType (SpecE E) _.
 
-Global Instance ReSum_FunStackE_E (E : EvType) (Γ : FunStack) : ReSum E (FunStackE E Γ) :=
-  fun e => inr (inr e).
+Global Instance EncodingType_SpecE E : EncodingType (SpecE E) := SpecERet E.
 
-Global Instance ReSumRet_FunStackE_E (E : EvType) Γ :
-  ReSumRet E (FunStackE E Γ) :=
+Global Instance ReSum_SpecE_E (E : EvType) : ReSum E (SpecE E) :=
+  fun e => Spec_vis (inr e).
+
+Global Instance ReSumRet_SpecE_E (E : EvType) : ReSumRet E (SpecE E) :=
   fun _ r => r.
 
-Global Instance ReSum_FunStackE_Error (E : EvType) (Γ : FunStack) : ReSum ErrorE (FunStackE E Γ) :=
-  fun e => inr (inl e).
+Global Instance ReSum_SpecE_Error (E : EvType) : ReSum ErrorE (SpecE E) :=
+  fun e => Spec_vis (inl e).
 
-Global Instance ReSumRet_FunStackE_Error (E : EvType) Γ :
-  ReSumRet ErrorE (FunStackE E Γ) :=
+Global Instance ReSumRet_SpecE_Error (E : EvType) : ReSumRet ErrorE (SpecE E) :=
   fun _ r => r.
-
-
-(* Embed a call in the top level of the FunStack into a FunStackE *)
-Global Instance ReSum_StackCall_FunStackE (E : EvType) (stack : FunStack) :
-  ReSum (StackCall stack) (FunStackE E stack) :=
-  fun args => inl args.
-
-(* Map the return value for embedding a call in the top level to a FunStackE *)
-Global Instance ReSumRet_StackCall_FunStackE E stack :
-  ReSumRet (StackCall stack) (FunStackE E stack) :=
-  fun _ r => r.
-
-Global Instance EncodingType_LRTInput stack lrt :
-  EncodingType (LRTInput stack lrt) := LRTOutput stack lrt.
-
-(* ReSum instances for embedding the nth LRTInput into a StackCall *)
-Global Instance ReSum_LRTInput_FunStackE E stack n :
-  ReSum (LRTInput stack (nthLRT stack n)) (FunStackE E stack) :=
-  fun args => resum (StackCallOfArgs stack n args).
-
-Global Instance ReSumRet_LRTInput_FunStackE E stack n :
-  ReSumRet (LRTInput stack (nthLRT stack n)) (FunStackE E stack) :=
-  fun _ r => r.
-
-Global Instance ReSum_Error_E_FunStack (E : EvType) (stack : FunStack) :
-  ReSum (SpecEvent (ErrorE + E)) (SpecEvent (FunStackE E stack)) :=
-  fun e => match e with
-           | Spec_vis e => Spec_vis (resum e)
-           | Spec_forall T => Spec_forall T
-           | Spec_exists T => Spec_exists T
-           end.
-
-Global Instance ReSumRet_Error_E_FunStack (E : EvType) (stack : FunStack) :
-  ReSumRet (SpecEvent (ErrorE + E)) (SpecEvent (FunStackE E stack)) :=
-  fun e =>
-    match e with
-    | Spec_vis e => fun x => resum_ret e x
-    | Spec_forall T => fun x => x
-    | Spec_exists T => fun x => x
-    end.
 
 
 (**
@@ -1308,44 +76,123 @@ Global Instance ReSumRet_Error_E_FunStack (E : EvType) (stack : FunStack) :
 
 (* The SpecM monad is an entree spec over FunStackE events *)
 Definition SpecM (E:EvType) stack A : Type :=
-  entree_spec (FunStackE E stack) A.
+  fixtree (SpecEv E) stack A.
 
-(* The observation / unfolding of a SpecM computation tree *)
-Definition SpecM' (E:EvType) stack A : Type :=
-  entree_spec' (FunStackE E stack) A.
+#[global] Instance Monad_SpecM {E stk} : Monad (SpecM E stk) := Monad_fixtree.
 
 (* The monadic operations on SpecM *)
-Definition RetS {E} {Γ A} (a : A) : SpecM E Γ A := ret a.
-Definition BindS {E} {Γ A B} (m : SpecM E Γ A) (k : A -> SpecM E Γ B) :=
+Definition RetS {E} {stk A} (a : A) : SpecM E stk A := ret a.
+Definition BindS {E} {stk A B} (m : SpecM E stk A) (k : A -> SpecM E stk B) :=
   bind m k.
-Definition IterS {E} {Γ A B} (body : A -> SpecM E Γ (A + B)) :
-  A -> SpecM E Γ B := EnTree.iter body.
-Definition AssumeS {E} {Γ} (P : Prop) : SpecM E Γ unit :=
-  assume_spec P.
-Definition AssertS {E} {Γ} (P : Prop) : SpecM E Γ unit :=
-  assert_spec P.
-Definition ForallS {E} {Γ} (A : Type) `{QuantType A} : SpecM E Γ A :=
-  forall_spec A.
-Definition ExistsS {E} {Γ} (A : Type) `{QuantType A} : SpecM E Γ A :=
-  exists_spec A.
-Definition TriggerS {E:EvType} {Γ} (e : E) : SpecM E Γ (encodes e) := trigger e.
-Definition ErrorS {E} {Γ} A (str : string) : SpecM E Γ A :=
-  bind (trigger (mkErrorE str)) (fun (x:Empty_set) => match x with end).
 
-Global Instance SpecM_Monad {E} Γ : Monad (SpecM E Γ) :=
-  {|
-    ret := fun A a => RetS a;
-    bind := fun A B m k => BindS m k;
-  |}.
+Definition ForallS {E} {stk} (A : Type) `{QuantType A} : SpecM E stk A :=
+  Fx_Vis (Spec_forall quantEnc : SpecEv E) (fun x => Fx_Ret (quantEnum x)).
+Definition ExistsS {E} {stk} (A : Type) `{QuantType A} : SpecM E stk A :=
+  Fx_Vis (Spec_exists quantEnc : SpecEv E) (fun x => Fx_Ret (quantEnum x)).
 
-Definition CallS {E stk R} (clos: LRTClos stk (LRT_SpecM R))
-  : SpecM E stk (LRTArg stk R) :=
-  eq_rect
-    (StackCallRet stk (LRTClosToCall stk R clos))
-    (SpecM E stk)
-    (trigger (LRTClosToCall stk R clos))
-    (LRTArg stk R)
-    (LRTClosToCallRet stk R clos).
+Definition AssumeS {E} {stk} (P : Prop) : SpecM E stk unit :=
+  BindS (ForallS P) (fun _ => ret tt).
+Definition AssertS {E} {stk} (P : Prop) : SpecM E stk unit :=
+  BindS (ExistsS P) (fun _ => ret tt).
+
+Definition TriggerS {E:EvType} {stk} (e : E) : SpecM E stk (encodes e) :=
+  Fx_Vis (resum e : SpecEv E) (fun x => Fx_Ret x).
+
+Definition ErrorS {E} {stk} A (str : string) : SpecM E stk A :=
+  Fx_Vis ((Spec_vis (inl (mkErrorE str))) : SpecEv E)
+    (fun (x:Empty_set) => match x with end).
+
+
+(**
+ ** Making and calling tpElems
+ **)
+
+(* An element of a type description that uses SpecM for the monadic type *)
+Fixpoint SpecElem E stk T : Type@{entree_u} :=
+  match T with
+  | Tp_M R => SpecM E stk (tpElem (SpecEv E) stk R)
+  | Tp_Pi A B => forall a, SpecElem E stk (B a)
+  | Tp_Arr A B =>
+      forall stk' (incl : stackIncl stk stk'),
+        tpElem (SpecEv E) stk' A -> SpecElem E stk' B
+  | Tp_SType A => tpElem (SpecEv E) stk (Tp_SType A)
+  | Tp_Pair A B => tpElem (SpecEv E) stk (Tp_Pair A B)
+  | Tp_Sum A B => tpElem (SpecEv E) stk (Tp_Sum A B)
+  | Tp_Sigma A B => tpElem (SpecEv E) stk (Tp_Sigma A B)
+  end.
+
+Definition PolySpecElem E stk T : Type@{entree_u} :=
+  forall stk' (incl : stackIncl stk stk'), SpecElem E stk' T.
+
+Fixpoint SpecElemToMonoInterp E stk T : SpecElem E stk T -> MonoInterp (SpecEv E) stk T :=
+  match T return SpecElem E stk T -> MonoInterp (SpecEv E) stk T with
+  | Tp_M R => fun elem args => elem
+  | Tp_Pi A B =>
+      fun elem args =>
+        SpecElemToMonoInterp E stk (B (projT1 args)) (elem (projT1 args)) (projT2 args)
+  | Tp_Arr A B =>
+      fun elem args =>
+        SpecElemToMonoInterp E stk B (elem stk (reflListIncl _) (fst args)) (snd args)
+  | Tp_SType A => fun elem args => match args with end
+  | Tp_Pair A B => fun elem args => match args with end
+  | Tp_Sum A B => fun elem args => match args with end
+  | Tp_Sigma A B => fun elem args => match args with end
+  end.
+
+Definition SpecElemToInterp E stk T (elem: PolySpecElem E stk T)
+  : FixTree.FxInterp (SpecEv E) stk T :=
+  fun stk' incl => SpecElemToMonoInterp E stk' T (elem stk' incl).
+
+Fixpoint InterpToSpecElem {E stk} T
+ : isFunTp T -> FxInterp (SpecEv E) stk T -> SpecElem E stk T :=
+  match T return isFunTp T -> FxInterp (SpecEv E) stk T -> SpecElem E stk T with
+  | Tp_M R => fun _ m => m stk (reflListIncl _) tt
+  | Tp_Pi A B => fun isfun f a =>
+                   InterpToSpecElem (B a) (isfun a)
+                     (fun stk' incl args => f stk' incl (existT _ a args))
+  | Tp_Arr A B =>
+      fun isfun f stk' incl arg =>
+        InterpToSpecElem B isfun (fun stk'' incl' args =>
+                                    f stk'' (compListIncl incl incl')
+                                      (liftTpElem incl' arg, args))
+  | Tp_SType _ => fun isfun => match isfun with end
+  | Tp_Pair _ _ => fun isfun => match isfun with end
+  | Tp_Sum _ _ => fun isfun => match isfun with end
+  | Tp_Sigma _ _ => fun isfun => match isfun with end
+  end.
+
+Definition callStkFun {E stk T} (stkf : StkFun stk T) : SpecElem E stk T :=
+  match stkf with
+  | MkStkFun _ _ n isn isfun =>
+      InterpToSpecElem T isfun
+        (fun stk' incl args =>
+           Fx_Call (MkStackCall _ _ T
+                      (applyListIncl incl n) (applyListInclNth incl isn) args)
+             (fun x => Fx_Ret x))
+  end.
+
+Fixpoint CallS {E stk T} : tpElem (SpecEv E) stk T -> SpecElem E stk T :=
+  match T return tpElem (SpecEv E) stk T -> SpecElem E stk T with
+  | Tp_M R =>
+      fun elem => match elem with
+                  | inl stkf => callStkFun stkf
+                  | inr m => embedEntree m
+                  end
+  | Tp_Pi A B =>
+      fun elem => match elem with
+                  | inl stkf => callStkFun stkf
+                  | inr f => fun a => CallS (f a)
+                  end
+  | Tp_Arr A B =>
+      fun elem => match elem with
+                  | inl stkf => callStkFun stkf
+                  | inr f => fun stk' incl arg => CallS (f stk' incl arg)
+                  end
+  | Tp_SType _ => fun elem => elem
+  | Tp_Pair _ _ => fun elem => elem
+  | Tp_Sum _ _ => fun elem => elem
+  | Tp_Sigma _ _ => fun elem => elem
+  end.
 
 
 (**
@@ -1876,6 +723,7 @@ End SpecMNotations.
  ** Interpreting SpecM computations in the state monad
  **)
 
+(*
 Section interpWithState.
 Import ExtLib.Structures.Functor.
 
@@ -1913,10 +761,10 @@ End interpWithState.
 
 (* Corecursively looks for performances of exceptional effects. If an
    exceptional performance is caught, then `catch` is performed instead. *)
-Program CoFixpoint try_catch {E:EvType} {Γ} {A} {B}
-    (is_exceptional : FunStackE E Γ -> option A)
-    (catch : A -> SpecM E Γ B) :
-    SpecM E Γ B -> SpecM E Γ B :=
+Program CoFixpoint try_catch {E:EvType} {stk} {A} {B}
+    (is_exceptional : FunStackE E stk -> option A)
+    (catch : A -> SpecM E stk B) :
+    SpecM E stk B -> SpecM E stk B :=
   fun t => match t with
   | go _ _ (RetF r) => ret r
   | go _ _ (TauF t') => Tau (try_catch is_exceptional catch t')
@@ -1931,3 +779,4 @@ Program CoFixpoint try_catch {E:EvType} {Γ} {A} {B}
       | Spec_exists T => Vis (Spec_exists T) (fun x => try_catch is_exceptional catch (k _))
       end
   end.
+*)
